Core_Erlang_Induction.v
@@ -24,238 +24,165 @@ Module Core_Erlang_Induction.
   end
   .
 
-  Section All.
-    Variable T : Type.
-    Variable P : T -> Prop.
-
-    Fixpoint All (ls : list T) : Prop :=
-      match ls with
-        | [ ] => True
-        | h::t => P h /\ All t
-      end.
-  End All.
-
-  Axiom Expression_ind2 : forall P : Expression -> Prop,
+  Check Expression_ind.
+  Axiom Expression_new_ind : forall P : Expression -> Prop,
        (forall l : Literal, P (ELiteral l)) ->
        (forall v : Var, P (EVar v)) ->
-       (forall f1 : Fun, P (EFunction f1)) ->
-       (forall hd : Expression, P hd -> forall tl : Expression, P tl -> P (EList hd tl)) ->
+       (forall f1 : FunctionSignature, P (EFunSig f1)) ->
+       (forall (vl : list Var) (e : Expression), P e -> P (EFun vl e)) ->
+       (forall hd : Expression,
+        P hd -> forall tl : Expression, P tl -> P (EList hd tl)) ->
        (forall l : list Expression, (forall e : Expression, In e l -> P e) -> P (ETuple l)) ->
-       (forall (f4 : FunctionSignature) (l : list Expression), (forall e : Expression, In e l -> P e) -> P (ECall f4 l)) ->
-       (forall (f5 : Var) (l : list Expression), (forall e : Expression, In e l -> P e) -> P (EApply f5 l)) ->
-       (forall (f6 : FunctionSignature) (l : list Expression), (forall e : Expression, In e l -> P e) -> P (EApplyTopLevel f6 l)) ->
-       (forall e : Expression, P e -> (forall l : list Clause, (forall cl : Clause, expr_clause_prop cl P) -> P (ECase e l))) ->
-       (forall (s : list Var) (el : list Expression) (e : Expression), (forall exp : Expression, In exp el -> P exp) -> P e -> P (ELet s el e)) ->
-       (forall (fnames : list FunctionSignature) (fs : list Fun) (e : Expression),
+       (forall (f5 : string) (l : list Expression), (forall e : Expression, In e l -> P e) -> P (ECall f5 l)) ->
+       (forall exp : Expression,
+        P exp -> forall l : list Expression, (forall e : Expression, In e l -> P e) -> P (EApply exp l)) ->
+       (forall e : Expression,
+        P e -> (forall l : list Clause, (forall cl : Clause, expr_clause_prop cl P) -> P (ECase e l))) ->
+       (forall (s : list Var) (el : list Expression) (e : Expression),
+        (forall e : Expression, In e el -> P e) -> P e -> P (ELet s el e)) ->
+       (forall (fnames : list FunctionSignature)
+          (fs : list (list Var * Expression)) (e : Expression),
         P e -> P (ELetrec fnames fs e)) ->
-       (forall kl vl : list Expression, (forall e : Expression, In e kl -> P e) -> (forall e : Expression, In e vl -> P e) -> P (EMap kl vl))
--> forall e : Expression, P e.
-  (*Variable P : Expression -> Prop.
+       (forall kl vl : list Expression,
+       (forall e : Expression, In e kl -> P e) -> (forall e : Expression, In e vl -> P e) -> P (EMap kl vl)) ->
+       forall e : Expression, P e.
 
-
-  Hypothesis literal_case : forall l, P (ELiteral l).
-  Hypothesis var_case : forall v : Var, P (EVar v).
-  Hypothesis function_case : forall f: Fun, P (EFunction f).
-  Hypothesis list_case : forall hd tl : Expression, P hd /\ P tl -> P (EList hd tl).
-  (*Hypothesis tuple_case : forall exps : list Expression, All Expression P exps -> P (ETuple exps).*)
-  Hypothesis tuple_case : forall exps : list Expression, All Expression P exps -> P (ETuple exps).
-  Hypothesis call_case : forall f exps, All Expression P exps -> P (ECall f exps).
-  Hypothesis apply_case : forall f exps, All Expression P exps -> P (EApply f exps).
-  Hypothesis top_apply_case : forall f exps, All Expression P exps -> P (EApplyTopLevel f exps).
-  Hypothesis let_case : forall sl el e, All Expression P el /\ P e -> P (ELet sl el e).
-  Hypothesis letrec_case : forall fnames fs e, P e -> P (ELetrec fnames fs e).
-  Hypothesis map_case : forall kl vl, All Expression P kl /\ All Expression P vl -> P (EMap kl vl).
-  
-  Fixpoint expr_induct (e : Expression) : P e :=
-    match e with
-     | ELiteral l => literal_case l
-     | EVar v => var_case v
-     | EFunction f => function_case f
-     | EList hd tl => list_case hd tl (conj (expr_induct hd) (expr_induct tl))
-     | ETuple l => tuple_case l ((fix list_ind (ls : list Expression) : All Expression P ls :=
-        match ls with
-        | [] => I
-        | x::xs => conj (expr_induct x) (list_ind xs)
-        end) l)
-     | ECall f l => call_case f l ((fix list_ind (ls : list Expression) : All Expression P ls :=
-        match ls with
-        | [] => I
-        | x::xs => conj (expr_induct x) (list_ind xs)
-        end) l)
-     | EApply f l => apply_case f l ((fix list_ind (ls : list Expression) : All Expression P ls :=
-        match ls with
-        | [] => I
-        | x::xs => conj (expr_induct x) (list_ind xs)
-        end) l)
-     | EApplyTopLevel f l => top_apply_case f l ((fix list_ind (ls : list Expression) : All Expression P ls :=
-        match ls with
-        | [] => I
-        | x::xs => conj (expr_induct x) (list_ind xs)
-        end) l)
-     | ELet s el e => let_case s el e (conj ((fix list_ind (ls : list Expression) : All Expression P ls :=
-        match ls with
-        | [] => I
-        | x::xs => conj (expr_induct x) (list_ind xs)
-        end) el) (expr_induct e))
-     | ELetrec fnames fs e => letrec_case fnames fs e (expr_induct e)
-     | EMap kl vl => map_case kl vl (conj (((fix list_ind (ls : list Expression) : All Expression P ls :=
-        match ls with
-        | [] => I
-        | x::xs => conj (expr_induct x) (list_ind xs)
-        end) kl)) (((fix list_ind (ls : list Expression) : All Expression P ls :=
-        match ls with
-        | [] => I
-        | x::xs => conj (expr_induct x) (list_ind xs)
-        end) vl)))
-    end.*)
-    
     Check eval_expr_ind.
 
 Axiom eval_expr_ind2
-     : forall P : Environment * Closures * Expression -> Expression -> Prop,
-       (forall (env : Environment) (s : Var) (cl : Closures),
-        P (env, cl, EVar s) (proj1_sig (get_value env (inl s)))) ->
-        
-        
-       (forall (env : Environment) (exprs1 exprs2 : list Expression) (cl : Closures),
-        Datatypes.length exprs1 = Datatypes.length exprs2 ->
-        (forall exp exp' : Expression,
-         In (exp, exp') (combine exprs1 exprs2) ->
-         (((env, cl, exp) -e> exp' /\ P (env, cl, exp) exp') \/ exp = exp') /\ exp' val) ->
-        ETuple exprs1 <> ETuple exprs2 -> P (env, cl, ETuple exprs1) (ETuple exprs2)) ->
-        
-        
-       (forall (env : Environment) (hd tl e' e'' : Expression) (cl : Closures),
-        (((env, cl, hd) -e> e' /\ P (env, cl, hd) e') \/ hd = e') /\ e' val ->
-        (((env, cl, tl) -e> e'' /\ P (env, cl, tl) e'') \/ tl = e'') /\ e'' val ->
-        EList hd tl <> EList e' e'' -> P (env, cl, EList hd tl) (EList e' e'')) ->
-        
-        
-        
-        (forall (env : Environment) (e e'' guard exp : Expression) (e' : Value) 
-          (cs : list Clause) (bindings : list (Var * Value)) (cl : Closures) 
-          (i : nat),
-        (env, cl, e) -e> proj1_sig e' /\ P (env, cl, e) (proj1_sig e') \/ e = proj1_sig e' ->
-        match_clause e' cs i = Some (guard, exp, bindings) ->
+     : forall P : Environment * Closures * Expression -> Value -> Prop,
+     
+     (* Literal *)
+       (forall (env : Environment) (l : Literal) (cl : Closures), 
+       P (env, cl, ELiteral l) (VLiteral l)) 
+       ->
+     (* Variable *)
+       (forall (env : Environment) (s : Var) (cl : Closures), 
+       P (env, cl, EVar s) (get_value env (inl s))) 
+       ->
+     (* Function name *)
+       (forall (env : Environment) (fsig : FunctionSignature) (cl : Closures),
+        P (env, cl, EFunSig fsig) (get_value env (inr fsig))) 
+        ->
+     (* Function definition *)
+       (forall (env : Environment) (vl : list Var) (e : Expression) (cl : Closures),
+        P (env, cl, EFun vl e) (VClosure env vl e)) 
+        ->
+     (* Tuple *)
+       (forall (env : Environment) (exps : list Expression) (vals : list Value) (cl : Closures),
+        Datatypes.length exps = Datatypes.length vals ->
+        (forall (exp : Expression) (val : Value),
+         In (exp, val) (combine exps vals) -> (env, cl, exp) -e> val) ->
+        (forall (exp : Expression) (val : Value),
+         In (exp, val) (combine exps vals) -> P (env, cl, exp) val) ->
+        P (env, cl, ETuple exps) (VTuple vals)) 
+        ->
+      (* List *)
+       (forall (env : Environment) (hd tl : Expression) (hdv tlv : Value) (cl : Closures),
+        (env, cl, hd) -e> hdv ->
+        P (env, cl, hd) hdv ->
+        (env, cl, tl) -e> tlv -> 
+        P (env, cl, tl) tlv -> 
+        P (env, cl, EList hd tl) (VList hdv tlv))
+        ->
+      (* Case *)
+       (forall (env : Environment) (e : Expression),
+        Expression ->
+        forall (guard exp : Expression) (v v' : Value) (cs : list Clause) (bindings : list (Var * Value))
+          (cl : Closures) (i : nat),
+        (env, cl, e) -e> v ->
+        P (env, cl, e) v ->
+        match_clause v cs i = Some (guard, exp, bindings) ->
         (forall j : nat,
          j < i ->
-         match_clause e' cs j = None \/
+         match_clause v cs j = None \/
          (forall (gg ee : Expression) (bb : list (Var * Value)),
-          match_clause e' cs j = Some (gg, ee, bb) ->
-          (add_bindings bb env, cl, gg) -e> ff /\ P (add_bindings bb env, cl, gg) ff \/ gg = ff)) ->
-        (add_bindings bindings env, cl, guard) -e> tt /\ P (add_bindings bindings env, cl, guard) tt \/ guard = tt ->
-        ((add_bindings bindings env, cl, exp) -e> e'' /\ P (add_bindings bindings env, cl, exp) e'' \/ exp = e'') /\ e'' val ->
-        P (env, cl, ECase e cs) e'') ->
-        
-       (*  (forall (env : Environment) (e e'' guard exp : Expression) (e' : Value) 
-          (cs : list Clause) (bindings : list (Var * Value)) (cl : Closures) 
-          (i : nat),
-        (env, cl, e) -e> proj1_sig e' /\ P (env, cl, e) (proj1_sig e') \/ e = proj1_sig e' ->
-        match_clause e' cs i = Some (guard, exp, bindings) ->
-        (forall j : nat,
-         j < i ->
-         match_clause e' cs j = None \/
-         (forall (gg ee : Expression) (bb : list (Var * Value)) (ee' : Expression),
-          match_clause e' cs j = Some (gg, ee, bb) ->
-          (((add_bindings bb env, cl, gg) -e> ee' /\ P (add_bindings bb env, cl, gg) ee' \/ gg = ee') /\ ee' <> tt))) ->
-        (add_bindings bindings env, cl, guard) -e> tt /\ P (add_bindings bindings env, cl, guard) tt \/ guard = tt ->
-        ((add_bindings bindings env, cl, exp) -e> e'' /\ P (add_bindings bindings env, cl, exp) e'' \/ exp = e'') /\ e'' val ->
-        P (env, cl, ECase e cs) e'') ->
-         *)
-        (* (forall (env : Environment) (e e'' guard exp : Expression) (e' : Value) 
-          (cs : list Clause) (bindings : list (Var * Value)) (cl : Closures),
-        ((env, cl, e) -e> proj1_sig e' /\ P (env, cl, e) (proj1_sig e')) \/ e = proj1_sig e' ->
-        match_clauses e' cs = Some (guard, exp, bindings) ->
-        (add_bindings bindings env, cl, guard) -e> tt \/ guard = tt ->
-        (((add_bindings bindings env, cl, exp) -e> e'' /\ P (add_bindings bindings env, cl, exp) e'') \/ exp = e'') /\ e'' val ->
-        P (env, cl, ECase e cs) e'') -> *)
-        
-        
-       (forall (env : Environment) (e' : Expression) (params exprs2 : list Expression)
-          (fname : FunctionSignature) (cl : Closures),
-        Datatypes.length params = Datatypes.length exprs2 ->
-        (forall exp exp' : Expression,
-         In (exp, exp') (combine params exprs2) ->
-         (((env, cl, exp) -e> exp' /\ P (env, cl, exp) exp') \/ exp = exp') /\ exp' val) ->
-        eval env fname exprs2 = e' /\ e' val -> P (env, cl, ECall fname params) e') ->
-        
-        
-        
-       (forall (exprs1 : list Expression) (exprs2 : list Value) (env : Environment)
-          (name : string) (args : nat) (e' : Expression) (cl : Closures),
-        Datatypes.length exprs1 = Datatypes.length exprs2 ->
-        Datatypes.length exprs1 = args ->
-        (forall (exp : Expression) (exp' : Value),
-         In (exp, exp') (combine exprs1 exprs2) ->
-         (((env, cl, exp) -e> proj1_sig exp' /\ P (env, cl, exp) (proj1_sig exp'))
-          \/ exp = proj1_sig exp')) ->
-        (((append_vars_to_env (get_vars (get_value env (inr (name, args)))) exprs2
-            (get_env_from_closure (inr (name, args)) cl), cl,
-         get_fun_exp (get_value env (inr (name, args)))) -e> e' /\ 
-         P (append_vars_to_env (get_vars (get_value env (inr (name, args)))) exprs2
-            (get_env_from_closure (inr (name, args)) cl), cl,
-         get_fun_exp (get_value env (inr (name, args)))) e')
-          \/
-         get_fun_exp (get_value env (inr (name, args))) = e') /\ e' val
-       ->
-        P (env, cl, EApplyTopLevel (name, args) exprs1) e') ->
-        
-        
-        
-       (forall (exprs1 : list Expression) (exprs2 : list Value) (env : Environment) 
-          (name : Var) (e' : Expression) (cl : Closures),
-        Datatypes.length exprs1 = Datatypes.length exprs2 ->
-        (forall (exp : Expression) (exp' : Value),
-         In (exp, exp') (combine exprs1 exprs2) ->
-         ((env, cl, exp) -e> proj1_sig exp' /\ P (env, cl, exp) (proj1_sig exp')) \/ exp = proj1_sig exp') ->
-        (((append_vars_to_env (get_vars (get_value env (inl name))) exprs2
-            (get_env_from_closure (inl name) cl), cl, get_fun_exp (get_value env (inl name))) -e>
-         e' /\  P (append_vars_to_env (get_vars (get_value env (inl name))) exprs2
-            (get_env_from_closure (inl name) cl), cl, get_fun_exp (get_value env (inl name))) e') \/ get_fun_exp (get_value env (inl name)) = e') /\ e' val 
-      ->
-        P (env, cl, EApply name exprs1) e') ->
-        
-        
-        
-       (forall (env : Environment) (exps : list Expression) (exprs2 : list Value)
-          (vars : list Var) (e e' : Expression) (cl : Closures),
-        Datatypes.length exprs2 = Datatypes.length exps ->
-        (forall (exp : Expression) (exp' : Value),
-         In (exp, exp') (combine exps exprs2) ->
-         (((env, cl, exp) -e> proj1_sig exp' /\ P (env, cl, exp) (proj1_sig exp')) \/ exp = proj1_sig exp')) ->
-        (((append_vars_to_env vars exprs2 env,
-         append_vars_to_closure vars (valuelist_to_exp exprs2) cl env, e) -e> e' /\  P (append_vars_to_env vars exprs2 env,
-         append_vars_to_closure vars (valuelist_to_exp exprs2) cl env, e) e' ) \/ 
-         e = e') /\ e' val 
-       ->
-          P (env, cl, ELet vars exps e) e') ->
-         
-         
-         
-         
-       (forall (env : Environment) (e e' : Expression) (fnames : list FunctionSignature)
-          (funs : list Fun) (cl : Closures),
+          match_clause v cs j = Some (gg, ee, bb) -> (add_bindings bb env, cl, gg) -e> ff 
+          (* Only this is additional *)
+          /\ P (add_bindings bb env, cl, gg) ff)) ->
+          (***)
+        (add_bindings bindings env, cl, guard) -e> tt ->
+        P (add_bindings bindings env, cl, guard) tt ->
+        (add_bindings bindings env, cl, exp) -e> v' ->
+        P (add_bindings bindings env, cl, exp) v' -> P (env, cl, ECase e cs) v') 
+        ->
+     (* Call *)
+       (forall (env : Environment) (v : Value) (params : list Expression) (vals : list Value)
+          (fname : string) (cl : Closures),
+        Datatypes.length params = Datatypes.length vals ->
+        (forall (exp : Expression) (val : Value),
+         In (exp, val) (combine params vals) -> (env, cl, exp) -e> val) ->
+        (forall (exp : Expression) (val : Value),
+         In (exp, val) (combine params vals) -> P (env, cl, exp) val) ->
+        eval env fname vals = v -> P (env, cl, ECall fname params) v)
+        ->
+     (* Apply variable *)
+       (forall (params : list Expression) (vals : list Value) (env app_env : Environment) 
+          (name : Var) (body : Expression) (v : Value) (var_list : list Var) 
+          (cl : Closures),
+        Datatypes.length params = Datatypes.length vals ->
+        (env, cl, EVar name) -e> VClosure app_env var_list body ->
+        P (env, cl, EVar name) (VClosure app_env var_list body) ->
+        (forall (exp : Expression) (val : Value),
+         In (exp, val) (combine params vals) -> (env, cl, exp) -e> val) ->
+        (forall (exp : Expression) (val : Value),
+         In (exp, val) (combine params vals) -> P (env, cl, exp) val) ->
+        (append_vars_to_env var_list vals (get_env_from_closure (inl name) cl), cl, body) -e> v ->
+        P (append_vars_to_env var_list vals (get_env_from_closure (inl name) cl), cl, body) v ->
+        P (env, cl, EApply (EVar name) params) v)
+        ->
+     (* Apply function name *)
+       (forall (params : list Expression) (vals : list Value) (env app_env : Environment)
+          (fsig : FunctionSignature) (body : Expression) (v : Value) (var_list : list Var)
+          (cl : Closures),
+        Datatypes.length params = Datatypes.length vals ->
+        (env, cl, EFunSig fsig) -e> VClosure app_env var_list body ->
+        P (env, cl, EFunSig fsig) (VClosure app_env var_list body) ->
+        (forall (exp : Expression) (val : Value),
+         In (exp, val) (combine params vals) -> (env, cl, exp) -e> val) ->
+        (forall (exp : Expression) (val : Value),
+         In (exp, val) (combine params vals) -> P (env, cl, exp) val) ->
+        (append_vars_to_env var_list vals (get_env_from_closure (inr fsig) cl), cl, body) -e> v ->
+        P (append_vars_to_env var_list vals (get_env_from_closure (inr fsig) cl), cl, body) v ->
+        P (env, cl, EApply (EFunSig fsig) params) v)
+        ->
+      (* Let *)
+       (forall (env : Environment) (exps : list Expression) (vals : list Value) 
+          (vars : list Var) (e : Expression) (v : Value) (cl : Closures),
+        Datatypes.length vals = Datatypes.length exps ->
+        (forall (exp : Expression) (val : Value),
+         In (exp, val) (combine exps vals) -> (env, cl, exp) -e> val) ->
+        (forall (exp : Expression) (val : Value),
+         In (exp, val) (combine exps vals) -> P (env, cl, exp) val) ->
+        (append_vars_to_env vars vals env, append_vars_to_closure vars vals cl env, e) -e> v ->
+        P (append_vars_to_env vars vals env, append_vars_to_closure vars vals cl env, e) v ->
+        P (env, cl, ELet vars exps e) v)
+        ->
+      (* Letrec *)
+       (forall (env : Environment) (e : Expression) (fnames : list FunctionSignature)
+          (funs : list (list Var * Expression)) (v : Value) (cl : Closures),
         Datatypes.length funs = Datatypes.length fnames ->
-        (((append_funs_to_env fnames funs env,
-         append_funs_to_closure fnames cl (append_funs_to_env fnames funs env), e) -e> e' /\ P (append_funs_to_env fnames funs env,
-         append_funs_to_closure fnames cl (append_funs_to_env fnames funs env), e) e') \/
-         e = e') /\ e' val
-         -> P (env, cl, ELetrec fnames funs e) e') ->
-         
-         
-         
-         
-         
-       (forall (kl vl : list Expression) (exprs2 : list Value) (env : Environment) (cl : Closures),
-        (forall exp : Expression, In exp kl -> exp val) ->
+        (append_funs_to_env fnames funs env,
+        append_funs_to_closure fnames cl (append_funs_to_env fnames funs env), e) -e> v ->
+        P
+          (append_funs_to_env fnames funs env,
+          append_funs_to_closure fnames cl (append_funs_to_env fnames funs env), e) v ->
+        P (env, cl, ELetrec fnames funs e) v)
+        ->
+     (* Map *)
+       (forall (kl vl : list Expression) (vvals kvals : list Value) (env : Environment) (cl : Closures),
         Datatypes.length vl = Datatypes.length kl ->
-        Datatypes.length vl = Datatypes.length exprs2 ->
-        (forall (exp : Expression) (exp' : Value),
-         In (exp, exp') (combine vl exprs2) ->
-         (((env, cl, exp) -e> proj1_sig exp' /\  P (env, cl, exp) (proj1_sig exp') \/ exp = proj1_sig exp'))) ->
-        P (env, cl, EMap kl vl) (EMap kl (valuelist_to_exp exprs2))) ->
-       forall (p : Environment * Closures * Expression) (e : Expression), p -e> e -> P p e.
-
-
+        Datatypes.length vl = Datatypes.length vvals ->
+        Datatypes.length vl = Datatypes.length kvals ->
+        (forall (exp : Expression) (val : Value),
+         In (exp, val) (combine kl kvals) -> (env, cl, exp) -e> val) ->
+        (forall (exp : Expression) (val : Value),
+         In (exp, val) (combine kl kvals) -> P (env, cl, exp) val) ->
+        (forall (exp : Expression) (val : Value),
+         In (exp, val) (combine vl vvals) -> (env, cl, exp) -e> val) ->
+        (forall (exp : Expression) (val : Value),
+         In (exp, val) (combine vl vvals) -> P (env, cl, exp) val) ->
+        P (env, cl, EMap kl vl) (VMap kvals vvals)) ->
+       forall (p : Environment * Closures * Expression) (v : Value), p -e> v -> P p v.
 
 End Core_Erlang_Induction.
