Core_Erlang_Proofs.v
@@ -16,23 +16,32 @@ Import ListNotations.
 Import Coq.Init.Logic.
 Import Omega.
 
-Lemma plus_comm_basic (e1 e2 : Expression) (env : Environment) : eval env ("plus"%string, 2) [e1 ; e2] = eval env ("plus"%string, 2) [e2; e1].
+Proposition plus_comm_basic (e1 e2 : Value) (env : Environment) : eval env "plus"%string [e1 ; e2] = eval env "plus"%string [e2; e1].
 Proof.
   simpl. case_eq e1; case_eq e2; intros.
-  1-169: try(reflexivity).
-  1-25: try(destruct l); try(destruct l0); try(reflexivity).
+  1-144: try(reflexivity).
+  1-23: try(destruct l); try(destruct l0); try(reflexivity).
   * rewrite <- Z.add_comm. reflexivity.
 Qed.
+
+Proposition and_comm_basic (e1 e2 : Value) (env : Environment) : eval env "and"%string [e1 ; e2] = eval env "and"%string [e2 ; e1].
+Proof.
+  simpl. case_eq e1; case_eq e2; intros.
+  1-144: try(reflexivity).
+  1-23: try(destruct l); try(destruct l0); try(reflexivity).
+  * pose (eqf := string_dec s "false"); pose (eqf2 := string_dec s0 "false"); pose (eqt := string_dec s "true"); pose (eqt2 := string_dec s0 "true"); destruct eqf, eqf2, eqt, eqt2; subst; try(reflexivity).
+    - admit.
+Admitted.
 
 Lemma ttt : forall p : Prop, True \/ p = True.
 Proof.
   auto.
 Qed.
 
-Lemma value_consistency : forall v : Value, (proj1_sig v) val.
+(* Lemma value_consistency : forall v : Value, (proj1_sig v) val.
 Proof.
   intros. pose (proj2_sig v). simpl in v0. exact v0.
-Qed.
+Qed. *)
 
 Theorem andd A B C : A -> B /\ C -> A -> B.
 Proof.
@@ -40,288 +49,12 @@ Proof.
 Qed.
 
 Lemma in_combined_list : forall P : Prop, forall l l' a b,
-  (forall e e' : Expression,
+  (forall e : Expression, forall e' : Value,
     In (e, e') ((a, b) :: combine l l') -> P) -> 
-  (forall e e' : Expression,
+  (forall e : Expression, forall e' : Value,
     In (e, e') (combine l l') -> P).
 Proof.
   intros. pose (in_cons (a, b) (e, e') (combine l l') H0). pose (H e e' i). assumption.
-Qed.
-
-Lemma trans_exp_list_equal : forall exprs exprs2 env cl,
-  (forall exp : Expression,
-    In exp exprs -> forall t : Expression, (env, cl, exp) -e> t -> False) ->
-  (forall exp exp' : Expression,
-     In (exp, exp') (combine exprs exprs2) -> ((env, cl, exp) -e> exp' \/ exp = exp') /\ exp' val) ->
-   length exprs = length exprs2 ->
-exprs = exprs2.
-Proof.
-  induction exprs; intros.
-  * inversion H1. apply eq_sym in H3. apply length_zero_iff_nil in H3. rewrite H3. reflexivity.
-  * inversion H1. apply eq_sym in H3. pose (element_exist Expression (Datatypes.length exprs) exprs2 H3). inversion e. inversion H2. rewrite H4 in *.
-  
-  (* exprs = x0 *)
-  pose (IHexprs x0 env cl). simpl combine in H0. assert (
-    forall exp exp' : Expression,
-     In (exp, exp') (combine exprs x0) ->
-     ((env, cl, exp) -e> exp' \/ exp = exp') /\ exp' val
-  ).
-  {
-    intros. pose (in_cons (a, x) (exp, exp') (combine exprs x0) H5). apply (H0 exp exp' i).
-  }
-  assert (
-    forall exp : Expression,
-    In exp (exprs) -> forall t : Expression, (env, cl, exp) -e> t -> False
-  ).
-  {
-    intros. pose (in_cons a exp exprs H6). apply (H exp i t). assumption.
-  }
-  inversion H1. pose (e0 H6 H5 H8). rewrite e1 in *.
-  (* a = x *)
-  pose (in_eq (a,x) (combine x0 x0)). pose (H0 a x i). inversion a0. inversion H7.
-  - pose (in_eq a x0). pose (H a i0). pose (f x H10). inversion f0.
-  - rewrite H10 in *. reflexivity.
-Qed.
-
-Lemma trans_val_list_equal : forall vl exprs2 env cl,
-  (forall exp : Expression,
-    In exp vl -> forall t : Expression, (env, cl, exp) -e> t -> False) ->
-  (forall (exp : Expression) (exp' : Value),
-      In (exp, exp') (combine vl exprs2) ->
-      (env, cl, exp) -e> proj1_sig exp' \/ exp = proj1_sig exp') ->
-   length vl = length exprs2 ->
-vl = valuelist_to_exp exprs2.
-Proof.
-  induction vl; intros.
-  * inversion H1. apply eq_sym in H3. apply length_zero_iff_nil in H3. rewrite H3. reflexivity.
-  * inversion H1. apply eq_sym in H3. pose (element_exist Value (Datatypes.length vl) exprs2 H3). inversion e. inversion H2. rewrite H4 in *.
-  
-  (* exprs = x0 *)
-  pose (IHvl x0 env cl). simpl combine in H0. assert (
-    forall exp exp',
-     In (exp, exp') (combine vl x0) ->
-     ((env, cl, exp) -e> proj1_sig exp' \/ exp = proj1_sig exp')
-  ).
-  {
-    intros. pose (in_cons (a, x) (exp, exp') (combine vl x0) H5). apply (H0 exp exp' i).
-  }
-  assert (
-    forall exp : Expression,
-    In exp (vl) -> forall t : Expression, (env, cl, exp) -e> t -> False
-  ).
-  {
-    intros. pose (in_cons a exp vl H6). apply (H exp i t). assumption.
-  }
-  inversion H1. pose (e0 H6 H5 H8). rewrite e1 in *.
-  (* a = x *)
-  pose (in_eq (a,x) (combine (valuelist_to_exp x0) x0)). pose (H0 a x i). inversion o.
-  - pose (in_eq a (valuelist_to_exp x0)). pose (H a i0). pose (f (proj1_sig x) H7). inversion f0.
-  - rewrite H7 in *. reflexivity.
-Qed.
-
-Theorem val_no_trans : forall v, v val -> (forall env cl t, ~ (env, cl, v) -e> t).
-Proof.
-  unfold not. intro v. intro H. intros env. intro cl. induction H; intros.
-  * inversion H.
-  * inversion H.
-  * inversion H1. subst. inversion H7. inversion H8. inversion H2.
-    - apply (IHValueJudgement1 e' H6).
-    - inversion H4.
-      + apply (IHValueJudgement2 e'' H10).
-      + subst. intuition.
-  * inversion H1. pose (trans_exp_list_equal exprs exprs2 env cl H0 H7 H5). rewrite e in *. intuition.
-  * inversion H1. pose (trans_val_list_equal vl exprs2 env cl H0 H10 H9). rewrite e in *. intuition.
-Qed.
-
-Lemma list_equality : 
-forall env cl, forall l l1 l2 : list Expression,
-(forall exp exp' : Expression,
-     In (exp, exp') (combine l l1) ->
-     ((env, cl, exp) -e> exp' /\
-      (forall v2 : Expression, (env, cl, exp) -e> v2 -> exp' = v2) \/ 
-      exp = exp') /\ exp' val) ->
-  
-(forall e e' : Expression, In (e, e') (combine l l2) -> ((env, cl, e) -e> e' \/ e = e') /\ e' val) ->
-
-length l = length l1 -> length l = length l2 ->
-
-l1 = l2.
-Proof.
-  intro. intro. intro. induction l; intros.
-  * inversion H1. inversion H2. apply eq_sym in H4. apply eq_sym in H5. apply length_zero_iff_nil in H4. apply length_zero_iff_nil in H5. subst. reflexivity.
-  * inversion H1. apply eq_sym in H4. pose (element_exist Expression (Datatypes.length l) l1 H4). inversion e. inversion H3. subst. inversion H2. apply eq_sym in H6. pose (element_exist Expression (Datatypes.length l) l2 H6). inversion e0. inversion H5. subst.
-  
-  pose (IHl x0 x2). simpl combine in H. simpl combine in H0. assert (
-    (* forall e e' : Expression,
-    In (e, e') (combine l x0) ->
-    ((env, cl, e) -e> e' \/ e = e') /\
-    e' val /\ (forall e2 : Expression, (env, cl, e) -e> e2 -> e' = e2)
-     *)
-    forall e e' : Expression,
-     In (e, e') (combine l x0) ->
-     ((env, cl, e) -e> e' /\
-      (forall e2 : Expression, (env, cl, e) -e> e2 -> e' = e2) \/ 
-      e = e') /\ e' val
-  ).
-  {
-    intros. pose (in_cons (a, x) (e2, e') (combine l x0) H7). apply (H e2 e' i).
-  }
-  assert (
-    forall e e' : Expression,
-     In (e, e') (combine l x2) -> ((env, cl, e) -e> e' \/ e = e') /\ e' val
-  ).
-  {
-    intros. pose (in_cons (a, x1) (e2, e') (combine l x2) H8). apply (H0 e2 e' i).
-  }
-  inversion H1. inversion H2.
-  pose (IHl x0 x2 H7 H8 H10 H11). rewrite e2 in *.
-  
-  
-  pose (H0 a x1). pose (H a x).
-  
-  simpl combine in a0.
-  pose (in_eq (a, x1) (combine l x2)). pose (a0 i). inversion a2.
-  
-  simpl combine in a1.
-  pose (in_eq (a, x) (combine l x2)). pose (a1 i0). inversion a3. inversion H13.
-    - inversion H15. inversion H9.
-      + pose (H17 x1 H18). rewrite e3. reflexivity.
-      + rewrite H18 in *. apply (val_no_trans x1 H12) in H16. inversion H16.
-    - rewrite H15 in *. inversion H9.
-      + apply (val_no_trans x H14) in H16. inversion H16.
-      + rewrite H16. reflexivity.
-Qed.
-
-(* Lemma val_unique : forall e e' : Expression, e val -> e' val ->  *)
-
-Axiom value_eq : forall v1 v2 : Value, proj1_sig v1 = proj1_sig v2 -> v1 = v2.
-
-Lemma val_list_equality : 
-forall env cl, forall l : list Expression, forall l1 l2 : list Value,
-(forall e e', In (e, e') (combine l l1) -> (
-  (env, cl, e) -e> proj1_sig e' \/ e = proj1_sig e') /\
-  
-  (forall e2 : Expression, (env, cl, e) -e> e2 -> proj1_sig e' = e2)) ->
-  
-(forall e e', In (e, e') (combine l l2) -> ((env, cl, e) -e> proj1_sig e' \/ e = proj1_sig e')) ->
-
-length l = length l1 -> length l = length l2 ->
-
-l1 = l2.
-Proof.
-  intro. intro. intro. induction l; intros.
-  * inversion H1. inversion H2. apply eq_sym in H4. apply eq_sym in H5. apply length_zero_iff_nil in H4. apply length_zero_iff_nil in H5. subst. reflexivity.
-  * inversion H1. apply eq_sym in H4. pose (element_exist Value (Datatypes.length l) l1 H4). inversion e. inversion H3. subst. inversion H2. apply eq_sym in H6. pose (element_exist Value (Datatypes.length l) l2 H6). inversion e0. inversion H5. subst.
-  
-  pose (IHl x0 x2). simpl combine in H. simpl combine in H0. assert (
-    forall e e',
-    In (e, e') (combine l x0) ->
-    ((env, cl, e) -e> proj1_sig e' \/ e = proj1_sig e') /\
-    (forall e2 : Expression, (env, cl, e) -e> e2 -> proj1_sig e' = e2)
-  ).
-  {
-    intros. pose (in_cons (a, x) (e2, e') (combine l x0) H7). apply (H e2 e' i).
-  }
-  assert (
-    forall e e',
-     In (e, e') (combine l x2) -> ((env, cl, e) -e> proj1_sig e' \/ e = proj1_sig e')
-  ).
-  {
-    intros. pose (in_cons (a, x1) (e2, e') (combine l x2) H8). apply (H0 e2 e' i).
-  }
-  inversion H1. inversion H2.
-  pose (IHl x0 x2 H7 H8 H10 H11). rewrite e2 in *.
-  
-  
-  pose (H0 a x1). pose (H a x).
-  
-  simpl combine in a0.
-  pose (in_eq (a, x) (combine l x2)). pose (a0 i). inversion a1.
-  
-  simpl combine in o.
-  pose (in_eq (a, x1) (combine l x2)). pose (o i0). inversion o0.
-  - pose (H12 (proj1_sig x1) H13). pose (value_eq x x1 e3). rewrite e4 in *. reflexivity.
-  - rewrite <- H13 in *. inversion H9.
-    + rewrite H13 in H14. pose (val_no_trans (proj1_sig x1) (proj2_sig x1) env cl (proj1_sig x) H14). inversion f. (*no_va_trans-zal menne*)
-    + rewrite H13 in *. pose (value_eq x1 x H14). rewrite e3. reflexivity.
-Qed.
-
-Lemma val_list_equality2 : 
-forall env cl, forall l : list Expression, forall l1 l2 : list Value,
-(forall (exp : Expression) (exp' : Value),
-  In (exp, exp') (combine l l1) ->
-  (env, cl, exp) -e> proj1_sig exp' /\
-  (forall v2 : Expression, (env, cl, exp) -e> v2 -> proj1_sig exp' = v2) \/
-  exp = proj1_sig exp') ->
-  
-(forall e e', In (e, e') (combine l l2) -> ((env, cl, e) -e> proj1_sig e' \/ e = proj1_sig e')) ->
-
-length l = length l1 -> length l = length l2 ->
-
-l1 = l2.
-Proof.
-  intro. intro. intro. induction l; intros.
-  * inversion H1. inversion H2. apply eq_sym in H4. apply eq_sym in H5. apply length_zero_iff_nil in H4. apply length_zero_iff_nil in H5. subst. reflexivity.
-  * inversion H1. apply eq_sym in H4. pose (element_exist Value (Datatypes.length l) l1 H4). inversion e. inversion H3. subst. inversion H2. apply eq_sym in H6. pose (element_exist Value (Datatypes.length l) l2 H6). inversion e0. inversion H5. subst.
-  
-  pose (IHl x0 x2). simpl combine in H. simpl combine in H0. assert (
-    (forall (e : Expression) (e' : Value),
-       In (e, e') (combine l x0) ->
-       (env, cl, e) -e> proj1_sig e' /\
-       (forall v2 : Expression, (env, cl, e) -e> v2 -> proj1_sig e' = v2) \/ 
-       e = proj1_sig e')
-  ).
-  {
-    intros. pose (in_cons (a, x) (e2, e') (combine l x0) H7). apply (H e2 e' i).
-  }
-  assert (
-    forall e e',
-     In (e, e') (combine l x2) -> ((env, cl, e) -e> proj1_sig e' \/ e = proj1_sig e')
-  ).
-  {
-    intros. pose (in_cons (a, x1) (e2, e') (combine l x2) H8). apply (H0 e2 e' i).
-  }
-  inversion H1. inversion H2.
-  pose (IHl x0 x2 H7 H8 H10 H11). rewrite e2 in *.
-  
-  
-  pose (o := H0 a x1). pose (H a x).
-  
-  simpl combine in o0.
-  pose (in_eq (a, x) (combine l x2)). pose (o0 i).
-  
-  simpl combine in o.
-  pose (in_eq (a, x1) (combine l x2)). pose (o i0).
-  inversion o1.
-  - inversion H9. inversion o2.
-    + pose (H13 (proj1_sig x1) H14). pose (value_eq x x1 e3). rewrite e4 in *. reflexivity.
-    + rewrite H14 in *. apply val_no_trans in H12. inversion H12. exact (proj2_sig x1).
-  - rewrite H9 in *. inversion o2.
-    + apply val_no_trans in H12. inversion H12. exact (proj2_sig x).
-    + apply value_eq in H12. rewrite H12. reflexivity.
-Qed.
-
-Proposition determinism_hypo env cl exp e'' v2:
-  (env, cl, exp) -e> e'' /\
-     (forall v2 : Expression, (env, cl, exp) -e> v2 -> e'' = v2) \/ 
-     exp = e''
-  ->
-  (env, cl, exp) -e> v2 \/ exp = v2
-  ->
-  e'' val
-  ->
-  v2 val
-->
-  e'' = v2
-.
-Proof.
-  intros. inversion H.
-  * inversion H3. inversion H0.
-    - pose (H5 v2 H6). assumption.
-    - subst. apply val_no_trans in H4. inversion H4. assumption.
-  * subst. inversion H0.
-    - apply val_no_trans in H3. inversion H3. assumption.
-    - subst. reflexivity.
 Qed.
 
 Import Omega.
@@ -332,249 +65,201 @@ Proof.
 intros. omega.
 Qed.
 
-Lemma index_case_equality (i i0 : nat) env0 cl0 cs e'0 guard guard0 exp exp0 bindings bindings0 : 
-  (forall j : nat,
-      j < i0 ->
-      match_clause e'0 cs j = None \/
-      (forall (gg ee : Expression) (bb : list (Var * Value)),
-       match_clause e'0 cs j = Some (gg, ee, bb) -> (add_bindings bb env0, cl0, gg) -e> ff \/ gg = ff))
+Proposition determinism_hypo env cl exp v1 v2: 
+ (env, cl, exp) -e> v1 ->
+ (forall v2 : Value, (env, cl, exp) -e> v2 -> v1 = v2)
   ->
+  (env, cl, exp) -e> v2
+->
+  v1 = v2
+.
+Proof.
+  intros. apply (H0 v2 H1).
+Qed.
+
+Lemma index_case_equality (i i0 : nat) env0 cl0 cs v guard guard0 exp exp0 bindings bindings0 : 
   (forall j : nat,
      j < i ->
-     match_clause e'0 cs j = None \/
+     match_clause v cs j = None \/
      (forall (gg ee : Expression) (bb : list (Var * Value)),
-      match_clause e'0 cs j = Some (gg, ee, bb) ->
+      match_clause v cs j = Some (gg, ee, bb) ->
       (add_bindings bb env0, cl0, gg) -e> ff /\
-      (forall v2 : Expression, (add_bindings bb env0, cl0, gg) -e> v2 -> ff = v2) \/ 
-      gg = ff))
+      (forall v2 : Value, (add_bindings bb env0, cl0, gg) -e> v2 -> ff = v2)))
   ->
-  match_clause e'0 cs i = Some (guard, exp, bindings)
+  (forall j : nat,
+      j < i0 ->
+      match_clause v cs j = None \/
+      (forall (gg ee : Expression) (bb : list (Var * Value)),
+       match_clause v cs j = Some (gg, ee, bb) -> (add_bindings bb env0, cl0, gg) -e> ff))
   ->
-  match_clause e'0 cs i0 = Some (guard0, exp0, bindings0)
+  match_clause v cs i = Some (guard, exp, bindings)
   ->
-  (add_bindings bindings0 env0, cl0, guard0) -e> tt \/ guard0 = tt
+  match_clause v cs i0 = Some (guard0, exp0, bindings0)
   ->
-  (add_bindings bindings env0, cl0, guard) -e> tt /\
-     (forall v2 : Expression, (add_bindings bindings env0, cl0, guard) -e> v2 -> tt = v2) \/
-     guard = tt
+  (add_bindings bindings0 env0, cl0, guard0) -e> tt
+  ->
+  (add_bindings bindings env0, cl0, guard) -e> tt 
+  ->
+  (forall v2 : Value, (add_bindings bindings env0, cl0, guard) -e> v2 -> tt = v2)
 ->
   i = i0.
 Proof.
   intros. pose (Nat.lt_decidable i i0). destruct d.
-  * pose (H i H5). inversion o.
-    - rewrite H6 in H1. inversion H1.
-    - pose (H6 guard exp bindings H1). pose (determinism_hypo (add_bindings bindings env0) cl0 guard tt ff H4 o0 (VJ_Literal (Atom "true")) (VJ_Literal (Atom "false"))). inversion e.
-  * apply not_lt in H5. apply (nat_ge_or) in H5. inversion H5.
+  * pose (H0 i H6). inversion o.
+    - rewrite H7 in *. inversion H1.
+    - pose (H7 guard exp bindings H1). pose (determinism_hypo (add_bindings bindings env0) cl0 guard tt ff H4 H5 e). inversion e0.
+  * apply not_lt in H6. apply (nat_ge_or) in H6. inversion H6.
     - assumption.
-    - pose (H0 i0 H6). inversion o.
-      + rewrite H7 in H2. inversion H2.
-      + pose (H7 guard0 exp0 bindings0 H2). inversion H3.
-        ** inversion o0.
-          -- inversion H9. pose (H11 tt H8). inversion e.
-          -- subst. apply val_no_trans in H8. inversion H8. exact (VJ_Literal (Atom "false")).
-        ** inversion o0.
-          -- subst. inversion H9. apply val_no_trans in H8. inversion H8. exact (VJ_Literal (Atom "true")).
-          -- subst. discriminate H9.
+    - pose (H i0 H7). inversion o.
+      + rewrite H8 in H2. inversion H2.
+      + pose (H8 guard0 exp0 bindings0 H2). inversion a. pose (H10 tt H3). inversion e.
+Qed.
+
+Lemma list_equality (env0 : Environment) (cl0 : Closures) (exps : list Expression)  : 
+forall vals vals0 : list Value,
+  (forall (exp : Expression) (val : Value),
+    In (exp, val) (combine exps vals) -> (env0, cl0, exp) -e> val) ->
+  (forall (exp : Expression) (val : Value),
+    In (exp, val) (combine exps vals) -> forall v2 : Value, (env0, cl0, exp) -e> v2 -> val = v2) ->
+  (forall (exp : Expression) (val : Value),
+    In (exp, val) (combine exps vals0) -> (env0, cl0, exp) -e> val) ->
+  Datatypes.length exps = Datatypes.length vals ->
+  Datatypes.length exps = Datatypes.length vals0
+->
+  vals = vals0.
+Proof.
+  induction exps.
+  * intros. inversion H3. inversion H2. apply eq_sym in H6. apply eq_sym in H5. apply length_zero_iff_nil in H6. apply length_zero_iff_nil in H5. subst. reflexivity.
+  * intros. inversion H3. inversion H2. 
+  
+  (* first elements are the same *)
+    pose (element_exist Value (Datatypes.length exps) vals (eq_sym H6)).
+    pose (element_exist Value (Datatypes.length exps) vals0 (eq_sym H5)).
+    inversion e. inversion e0. inversion H4. inversion H7. subst.
+    pose (in_eq (a, x) (combine (exps) (x1))).
+    pose (in_eq (a, x0) (combine (exps) (x2))).
+    pose (H1 a x0 i0).
+    pose (H0 a x i x0 e1). rewrite <- e2 in *.
+  (* remaining lists are the same *)
+  
+  (* These three asserts ensure, that if something states for every element in a (b::l) list, then it states
+  for every element in l too*)
+    assert (
+      forall (exp : Expression) (val : Value),
+       In (exp, val) (combine exps x1) ->
+       forall v2 : Value, (env0, cl0, exp) -e> v2 -> val = v2
+    ).
+    {
+      intros. pose (in_cons (a, x) (exp, val) (combine exps x1) H8). pose (H0 exp val i1 v2 H9). assumption.
+    }
+    assert (
+      forall (exp : Expression) (val : Value),
+    In (exp, val) (combine exps x1) -> (env0, cl0, exp) -e> val
+    ).
+    {
+      intros. pose (in_cons (a, x) (exp, val) (combine exps x1) H9). pose (H exp val i1). assumption.
+    }
+    assert (
+      forall (exp : Expression) (val : Value),
+     In (exp, val) (combine exps x2) -> (env0, cl0, exp) -e> val
+    ).
+    {
+      intros. pose (in_cons (a, x0) (exp, val) (combine exps x2) H10). pose (H1 exp val i1). assumption.
+    }
+    (* simpl list lengths *)
+    inversion H2.
+    inversion H3.
+    pose (IHexps x1 x2 H9 H8 H10 H12 H13). rewrite e3.
+    reflexivity.
 Qed.
 
 Theorem determinism : forall env cl e v1, (env, cl, e) -e> v1 -> (forall v2, (env, cl, e) -e> v2 -> v1 = v2).
 Proof.
   intro. intro. intro. intro. intro H. induction H using eval_expr_ind2.
-  (* VARIABLE *)
-  * intros. inversion H. reflexivity.
+  (* LITERAL, VARIABLE, FUNCTION NAME, FUNCTION DEFINITION *)
+  1-4: intros; inversion H; reflexivity.
 
   (* TUPLE *)
-  * intros. case_eq (combine exprs1 exprs2).
-    - intros. inversion H2. pose (combine_split exprs1 exprs2 H). pose (combine_split exprs1 exprs3 H7). rewrite H3 in *. inversion e0. subst. intuition.
-    - intros. inversion H2. subst. pose (list_equality env0 cl0 exprs1 exprs2 exprs3 H0 H9 H H7). rewrite e0 in *. reflexivity.
+  * intros. inversion H2. subst. pose (list_equality env0 cl0 exps vals vals0 H0 H1 H8 H H7). rewrite e0. reflexivity.
 
   (* LIST *)
-  * intros. inversion H. inversion H0. inversion H2. subst. inversion H12. inversion H13. 
-  pose (e0 := determinism_hypo env0 cl0 hd e' e'0 H3 H7 H4 H8). rewrite e0.
-  pose (e1 := determinism_hypo env0 cl0 tl e'' e''0 H5 H9 H6 H10). rewrite e1. reflexivity.
-  
+  * intros. inversion H1. subst. rewrite (IHeval_expr1 hdv0 H7). rewrite (IHeval_expr2 tlv0 H8). reflexivity.
+
   (* CASE *)
   * intros. inversion H4. subst.
-    pose (determinism_hypo env0 cl0 e0 (proj1_sig e') (proj1_sig e'0) H H9 (proj2_sig e') (proj2_sig e'0)). apply value_eq in e1. rewrite e1 in *.
-    pose (index_case_equality i i0 env0 cl0 cs e'0 guard guard0 exp exp0 bindings bindings0 H12 H1 H0 H10 H13 H2).
-    (** Why is this neccessary????????????????????? *)
-     assert (match_clause e'0 cs i = Some (guard, exp, bindings)). assumption. rewrite e2 in H5.
-     assert (match_clause e'0 cs i0 = Some (guard0, exp0, bindings0)). assumption. rewrite H5 in H6.
-    (** end *)
-     inversion H6. rewrite H8, H11, H15 in *. inversion H14. inversion H3.
-     pose (determinism_hypo
-              (add_bindings bindings0 env0)
-              cl0
-              exp0
-              e''
-              v2
-              H17 H7 H18 H16
-     ). assumption.
+    (* determinism of initial expression *)
+    rewrite <- (IHeval_expr1 v0 H9) in *.
+    (* determinism of clause selection (i = i0) *)
+    pose (index_case_equality i i0 env0 cl0 cs v guard guard0 exp exp0 bindings bindings0 H1 H12 H0 H10 H13 H2 IHeval_expr2). 
+    (* Coq Hacking for possible rewrites *)
+    pose H10. rewrite <- e1 in e2. pose H0. rewrite e2 in e3. inversion e3. rewrite H6, H7, H8 in *.
+    (* clause evaluation *)
+    pose (IHeval_expr3 v2 H14). assumption.
 
   (* CALL *)
-  * intros. case_eq (combine params exprs2).
-    - intros. inversion H2. pose (combine_split params exprs2 H). pose (combine_split params exprs0 H9). rewrite H3 in *. inversion e0. subst. inversion H1. inversion H11. inversion H9. apply eq_sym in H12. apply length_zero_iff_nil in H12. subst. reflexivity.
-    - intros. inversion H2. pose (list_equality env0 cl0 params exprs2 exprs0 H0 H10 H H9). rewrite e0 in *. inversion H1. inversion H11. rewrite <- H12. rewrite <- H14. reflexivity.
+  * intros. inversion H3. subst. pose (list_equality env0 cl0 params vals vals0 H0 H1 H10 H H9). rewrite e0. reflexivity.
 
-  (* TOP LEVEL APPLY *)
-  * intros. case_eq (combine exprs1 exprs2).
-    - intros. inversion H3. subst. pose (combine_split exprs1 exprs3 H11). pose (combine_split exprs1 exprs2 H). rewrite H4 in *. inversion e1. subst. inversion H11. apply eq_sym in H5. apply length_zero_iff_nil in H5. subst. simpl in *. inversion H14. inversion H2.
-    pose (determinism_hypo 
-          (append_vars_to_env (get_vars (get_value env0 (inr (name, 0)))) []
-            (get_env_from_closure (inr (name, 0)) cl0)) 
-          cl0
-          (get_fun_exp (get_value env0 (inr (name, 0))))
-          e'
-          v2
-          H6 H0 H7 H5). assumption.
-    - intros. inversion H3. subst. pose (val_list_equality2 env0 cl0 exprs1 exprs2 exprs3 H1 H13 H H11). rewrite e0 in *. inversion H2. inversion H14.
-    pose (determinism_hypo 
-          (append_vars_to_env (get_vars (get_value env0 (inr (name, Datatypes.length exprs1)))) exprs3
-            (get_env_from_closure (inr (name, Datatypes.length exprs1)) cl0)) 
-          cl0 
-          (get_fun_exp (get_value env0 (inr (name, Datatypes.length exprs1)))) 
-          e' 
-          v2 
-          H0 H6 H5 H7). assumption.
-        
-  (* APPLY *)
-  * intros. case_eq (combine exprs1 exprs2).
-    - intros. inversion H2. subst. pose (combine_split exprs1 exprs3 H9). pose (combine_split exprs1 exprs2 H). rewrite H3 in *. inversion e1. subst. inversion H9. apply eq_sym in H5. apply length_zero_iff_nil in H5. subst. simpl in *. inversion H11. inversion H1. 
-    pose (determinism_hypo 
-            (append_vars_to_env (get_vars (get_value env0 (inl name))) []
-             (get_env_from_closure (inl name) cl0))
-            cl0
-            (get_fun_exp (get_value env0 (inl name)))
-            e'
-            v2
-            H6 H4 H7 H5). assumption.
-    - intros. inversion H2. subst. pose (val_list_equality2 env0 cl0 exprs1 exprs2 exprs3 H0 H10 H H9). rewrite e0 in *. inversion H11. inversion H1. 
-    pose (determinism_hypo
-            (append_vars_to_env (get_vars (get_value env0 (inl name))) exprs3
-               (get_env_from_closure (inl name) cl0))
-            cl0
-            (get_fun_exp (get_value env0 (inl name)))
-            e'
-            v2
-            H6 H4 H7 H5
-         ). assumption.
+  (* APPLY VAR *)
+  * intros. inversion H4. subst. pose (list_equality env0 cl0 params vals vals0 H1 H2 H12 H H9). rewrite e0 in *.
+   (* The equality of the var lists *)
+   pose (IHeval_expr1 (VClosure app_env0 var_list0 body0) H11). inversion e1. rewrite H6, H7, H8 in *.
+   (* equality of the expressions *)
+   pose (IHeval_expr2 v2 H13). assumption.
+
+  (* APPLY FUNNAME *)
+  * intros. inversion H4. subst. pose (list_equality env0 cl0 params vals vals0 H1 H2 H12 H H9). rewrite e0 in *.
+   (* The equality of the var lists *)
+   pose (IHeval_expr1 (VClosure app_env0 var_list0 body0) H11). inversion e1. rewrite H6, H7, H8 in *.
+   (* equality of the expressions *)
+   pose (IHeval_expr2 v2 H13). assumption.
   
   (* LET *)
-  * intros. case_eq (combine exps exprs2).
-    - intros. inversion H2. subst. apply eq_sym in H10. apply eq_sym in H. pose (combine_split exps exprs0 H10). pose (combine_split exps exprs2 H). rewrite H3 in *. inversion e2. subst. inversion H10. apply eq_sym in H5. apply length_zero_iff_nil in H5. subst. simpl in *. inversion H12. inversion H1. 
-    pose (determinism_hypo
-             (append_vars_to_env vars [] env0)
-             (append_vars_to_closure vars [] cl0 env0)
-             e0
-             e'
-             v2
-             H6 H4 H7 H5
-    ). assumption.
-    - intros. inversion H2. subst. pose (val_list_equality2 env0 cl0 exps exprs2 exprs0 H0 H11 (eq_sym H) (eq_sym H10)). rewrite e1 in *. inversion H1. inversion H12.
-    pose (determinism_hypo
-             (append_vars_to_env vars exprs0 env0)
-             (append_vars_to_closure vars (valuelist_to_exp exprs0) cl0 env0)
-             e0
-             e'
-             v2
-             H4 H6 H5 H7
-    ). assumption.
+  * intros. inversion H3. subst. pose (list_equality env0 cl0 exps vals vals0 H0 H1 H11 (eq_sym H) (eq_sym H10)). rewrite e1 in *.
+   pose (IHeval_expr v2 H12). assumption.
 
   (* LETREC *)
-  * intros. inversion H0. inversion H1. subst. inversion H11. 
-    pose (determinism_hypo
-             (append_funs_to_env fnames funs env0)
-             (append_funs_to_closure fnames cl0 (append_funs_to_env fnames funs env0))
-             e0
-             e'
-             v2
-             H2 H4 H3 H5
-    ). assumption.  
+  * intros. inversion H1. subst. pose (IHeval_expr v2 H9). assumption.
   
   (* MAP *)
-  * intros. case_eq (combine vl exprs2).
-    - intros. inversion H3. pose (combine_split vl exprs2 H1). pose (combine_split vl exprs0 H12). rewrite H4 in *. inversion e0. subst. inversion H10. apply eq_sym in H6. apply length_zero_iff_nil in H6. subst. inversion H12. apply eq_sym in H6. apply length_zero_iff_nil in H6. subst. reflexivity.
-    - intros. inversion H3. subst. pose (val_list_equality2 env0 cl0 vl exprs2 exprs0 H2 H13 H1 H12). rewrite e0 in *. reflexivity.
-Qed.
-
-Example call_comm : forall e e'  v v' cl env t,  
-  (e = v \/ (env, cl, e) -e> v) /\ v val -> 
-  (e' = v' \/ (env, cl, e') -e> v') /\ v' val ->
-  (env, cl, ECall ("plus"%string, 2) [e ; e']) -e> t ->
-  (env, cl, ECall ("plus"%string, 2) [e' ; e]) -e> t.
-Proof.
-  intros. inversion H1. inversion H9.
-  subst. simpl in H7. pose (element_exist Expression 1 exprs2 (eq_sym H7)). inversion e0. inversion H2. subst. inversion H7. pose (element_exist Expression 0 x0 (eq_sym H4)). inversion e1. inversion H3. subst. inversion H4. apply eq_sym in H6. apply length_zero_iff_nil in H6. rewrite H6 in *. assert ([x; x1] = [v ; v']).
-  * pose (H8 e x). simpl combine in a. pose (in_eq (e,x) [(e', x1)]). pose (a i). inversion a0.
-  inversion H5.
-    - inversion H. inversion H13.
-      + subst. pose (val_no_trans v H14 env cl x H12). inversion f.
-      + pose (determinism env cl e v H15 x H12). rewrite e2 in *. inversion H0. assert (In (e', x1) (combine [e; e'] [x; x1])).
-      {
-        simpl. auto.
-      }
-      pose (H8 e' x1 H18 ). inversion a1. inversion H16.
-      ** rewrite H21 in *. inversion H19.
-        -- apply val_no_trans in H22. inversion H22. exact H17.
-        -- rewrite H22. reflexivity.
-      ** inversion H19.
-        -- pose (determinism env cl e' v' H21 x1 H22). rewrite e3 in *. reflexivity.
-        -- rewrite H22 in *. apply val_no_trans in H21. inversion H21. exact H20.
-    - subst. inversion H. inversion H6.
-      + subst. inversion H0. assert (In (e', x1) (combine [v; e'] [v; x1])). { simpl. auto. } pose (H8 e' x1 H15). inversion a1. inversion H13.
-        ** inversion H16.
-          -- rewrite H18 in H19. apply val_no_trans in H19. inversion H19. assumption.
-          -- subst. reflexivity.
-        ** inversion H16.
-          -- pose (determinism env cl e' v' H18 x1 H19). rewrite e in *. reflexivity.
-          -- subst. apply val_no_trans in H18. inversion H18. assumption.
-      + apply val_no_trans in H13. inversion H13. exact H10.
-
-  * subst. apply eval_call with (exprs2 := [x1; x]).
-    - reflexivity.
-    - intros. inversion H6.
-      + inversion H10.  rewrite H13 in *. rewrite H14 in *. assert (In (exp, exp') (combine [e; exp] [x; exp'])). { simpl. auto. } pose (H8 exp exp' H12). assumption.
-      + inversion H10.
-        ** inversion H12. rewrite H15 in *. rewrite H14 in *. assert (In (exp, exp') (combine [exp; e'] [exp'; x1])). { simpl. intuition. } pose (H8 exp exp' H13). assumption.
-        ** inversion H12.
-    - split.
-      + apply plus_comm_basic.
-      + assumption.
+  * intros. inversion H6. subst.
+  (* Key list equality *)
+  rewrite H in *.
+  pose (list_equality env0 cl0 kl kvals kvals0 H2 H3 H15 H1 H14). rewrite e0 in *.
+  (* value list equality *)
+  rewrite <- H in *.
+  pose (list_equality env0 cl0 vl vvals vvals0 H4 H5 H16 H0 H12). rewrite e1 in *.
+  reflexivity.
 Qed.
 
 Ltac unfold_list exprs2 n H1 name :=
 subst; simpl in H1; pose (name := element_exist Expression n exprs2 (eq_sym H1)); inversion name; inversion H0.
 
-
-Example call_comm2 : forall e e' cl env t,
-  (env, cl, ECall ("plus"%string, 2) [e ; e']) -e> t <->
-  (env, cl, ECall ("plus"%string, 2) [e' ; e]) -e> t.
+Example call_comm : forall e e' cl env t,
+  (env, cl, ECall "plus"%string [e ; e']) -e> t <->
+  (env, cl, ECall "plus"%string [e' ; e]) -e> t.
 Proof.
-  split.
-  * intros. inversion H. subst. inversion H7. simpl in H5. pose (element_exist Expression 1 exprs2 (eq_sym H5)). inversion e0. inversion H2. subst. inversion H5. pose (element_exist Expression 0 x0 (eq_sym H3)). inversion e1.  inversion H0. inversion H3. rewrite H4 in *. inversion H9. apply eq_sym in H10. apply length_zero_iff_nil in H10. subst.
-  apply eval_call with (exprs2 := [x1; x]).
-  - reflexivity.
-  - intros. inversion H4.
-    + inversion H8. subst. apply (H6 exp exp'). simpl. auto.
-    + inversion H8.
-      ** inversion H10. subst. apply (H6 exp exp'). simpl. auto.
-      ** inversion H10.
-  - split.
-    + apply plus_comm_basic.
-    + assumption.
-
-  (* copy paszta *)
-  * intros. inversion H. subst. inversion H7. simpl in H5. pose (element_exist Expression 1 exprs2 (eq_sym H5)). inversion e0. inversion H2. subst. inversion H5. pose (element_exist Expression 0 x0 (eq_sym H3)). inversion e1.  inversion H0. inversion H3. rewrite H4 in *. inversion H9. apply eq_sym in H10. apply length_zero_iff_nil in H10. subst.
-  apply eval_call with (exprs2 := [x1; x]).
-  - reflexivity.
-  - intros. inversion H4.
-    + inversion H8. subst. apply (H6 exp exp'). simpl. auto.
-    + inversion H8.
-      ** inversion H10. subst. apply (H6 exp exp'). simpl. auto.
-      ** inversion H10.
-  - split.
-    + apply plus_comm_basic.
-    + assumption.
+  intros. split.
+  (* List elements *)
+  1-2: intros; inversion H; subst; simpl in H5; pose (element_exist Value 1 vals (eq_sym H5)); inversion e0; inversion H0; subst; simpl in H5; inversion H5; pose (element_exist Value 0 x0 (eq_sym H2)); inversion e1; inversion H1; subst; simpl in H5; inversion H5; apply eq_sym in H4; apply length_zero_iff_nil in H4; subst;
+  (* eqivalence *)
+  apply eval_call with ([x1;x]).
+    1, 4: reflexivity.
+    1, 3: intros.
+    { inversion H3.
+        inversion H4. rewrite H8, H9 in *. apply H6. simpl. intuition.
+        
+        inversion H4.
+        inversion H7. rewrite H9, H10 in *. apply H6. simpl. intuition.
+        inversion H7.
+      }
+    2, 3 : apply plus_comm_basic.
+    { inversion H3.
+        inversion H4. rewrite H8, H9 in *. apply H6. simpl. intuition.
+        
+        inversion H4.
+        inversion H7. rewrite H9, H10 in *. apply H6. simpl. intuition.
+        inversion H7.
+      }
 Qed.
 
 End Core_Erlang_Proofs.
